FinitePerm/Congr.lean
@@ -4,26 +4,26 @@ Released under Apache 2.0 license as described in the file LICENSE.
 Authors: Wrenna Robson
 -/
 module
-public import Finperm.HMul
-public import Finperm.MinPerm
+public import FinitePerm.HMul
+public import FinitePerm.MinPerm
 
 @[expose] public section
 
-namespace Finperm
+namespace PermVector
 
-def IsCongr {n m : Nat} (a : Finperm n) (b : Finperm m) : Prop :=
+def IsCongr {n m : Nat} (a : PermVector n) (b : PermVector m) : Prop :=
   (∃ (h : n ≤ m), a.castGE h = b) ∨ (∃ (h : m ≤ n), b.castGE h = a)
 
 section IsCongr
 
-variable {n m l i : Nat} {a : Finperm n} {b : Finperm m} {c : Finperm l}
+variable {n m l i : Nat} {a : PermVector n} {b : PermVector m} {c : PermVector l}
 
 theorem isCongr_pointwise :
     a.IsCongr b ↔ (∀ i (hin : i < n) (him : i < m), a[i] = b[i]) ∧
     (∀ i, ∀ (hi : i < n), m ≤ i → a[i] = i) ∧
     (∀ i, ∀ (hi : i < m), n ≤ i → b[i] = i) := by
   unfold IsCongr
-  simp only [Finperm.ext_iff, getElem_castGE]
+  simp only [PermVector.ext_iff, getElem_castGE]
   grind
 
 theorem IsCongr.eq_castGE_of_le (h : n ≤ m) (hab : a.IsCongr b) : a.castGE h = b :=
@@ -48,7 +48,7 @@ grind_pattern castGE_isCongr => a.castGE h
 
 @[simp, grind =] theorem castGE_eq_iff {h : n ≤ k} {h'} :
     a.castGE h = b.castGE h' ↔ a.IsCongr b := by
-  simp only [Finperm.ext_iff, getElem_castGE, isCongr_pointwise]
+  simp only [PermVector.ext_iff, getElem_castGE, isCongr_pointwise]
   grind
 
 @[simp, grind =] theorem isCongr_castGE_castGE_iff {h : n ≤ k} {h' : m ≤ o} :
@@ -56,18 +56,18 @@ grind_pattern castGE_isCongr => a.castGE h
   simp only [isCongr_pointwise, getElem_castGE, dite_eq_right_iff]
   grind
 
-instance {a : Finperm n} {b : Finperm m} : Decidable (a.IsCongr b) :=
+instance {a : PermVector n} {b : PermVector m} : Decidable (a.IsCongr b) :=
   decidable_of_decidable_of_iff isCongr_pointwise.symm
 
-theorem IsCongr.eq {a' : Finperm n} (h : a.IsCongr a') : a = a' :=
+theorem IsCongr.eq {a' : PermVector n} (h : a.IsCongr a') : a = a' :=
   (h.eq_castGE_of_ge n.le_refl).symm.trans a'.castGE_refl
 
-@[simp] theorem isCongr_refl (a : Finperm n) : a.IsCongr a :=
+@[simp] theorem isCongr_refl (a : PermVector n) : a.IsCongr a :=
   isCongr_of_castGE_eq_right n.le_refl a.castGE_refl
 
 theorem isCongr_rfl : a.IsCongr a := isCongr_refl a
 
-@[simp, grind =] theorem isCongr_iff_eq {a' : Finperm n} : a.IsCongr a' ↔ a = a' :=
+@[simp, grind =] theorem isCongr_iff_eq {a' : PermVector n} : a.IsCongr a' ↔ a = a' :=
   ⟨IsCongr.eq, Eq.rec a.isCongr_refl⟩
 
 @[grind →] theorem IsCongr.symm (hab : a.IsCongr b) : b.IsCongr a := hab.elim Or.inr Or.inl
@@ -80,7 +80,7 @@ theorem isCongr_comm : a.IsCongr b ↔ b.IsCongr a := by grind
 @[grind →] theorem IsCongr.inv_inv : a.IsCongr b → a⁻¹.IsCongr b⁻¹ :=
   Or.imp (Exists.imp <| by simp) (Exists.imp <| by simp)
 
-theorem IsCongr.mul_mul {a' : Finperm n} {b' : Finperm m} (hab : a.IsCongr b)
+theorem IsCongr.mul_mul {a' : PermVector n} {b' : PermVector m} (hab : a.IsCongr b)
     (hab' : a'.IsCongr b') : (a * a').IsCongr (b * b') := by
   rcases hab  <;> rcases hab' <;> grind
 
@@ -94,18 +94,18 @@ theorem IsCongr.congrLeft (hab : a.IsCongr b) : a.IsCongr c ↔ b.IsCongr c := b
 theorem IsCongr.congrRight (hab : a.IsCongr b) : c.IsCongr a ↔ c.IsCongr b := by grind
 
 @[grind .]
-theorem isCongr_one_one : (1 : Finperm n).IsCongr (1 : Finperm m) :=
+theorem isCongr_one_one : (1 : PermVector n).IsCongr (1 : PermVector m) :=
   (Nat.le_or_ge n m).elim (fun _ => .inl (by grind)) (fun _ => .inr (by grind))
 
-@[grind =>] theorem IsCongr.eq_one (ha : a.IsCongr (1 : Finperm m)) : a = 1 := by
+@[grind =>] theorem IsCongr.eq_one (ha : a.IsCongr (1 : PermVector m)) : a = 1 := by
   rcases ha <;> grind
 
-@[grind =>] theorem IsCongr.one_eq (ha : (1 : Finperm m).IsCongr a) : 1 = a := by
+@[grind =>] theorem IsCongr.one_eq (ha : (1 : PermVector m).IsCongr a) : 1 = a := by
   rcases ha <;> grind
 
-@[simp] theorem isCongr_one_iff : a.IsCongr (1 : Finperm m) ↔ a = 1 := by grind
+@[simp] theorem isCongr_one_iff : a.IsCongr (1 : PermVector m) ↔ a = 1 := by grind
 
-@[simp] theorem one_isCongr_iff : (1 : Finperm m).IsCongr a ↔ a = 1 := by grind
+@[simp] theorem one_isCongr_iff : (1 : PermVector m).IsCongr a ↔ a = 1 := by grind
 
 theorem IsCongr.inv_right (hab : a.IsCongr b⁻¹) : a⁻¹.IsCongr b := by grind
 
@@ -123,19 +123,19 @@ grind_pattern isCongr_cast => a.cast h
 
 grind_pattern cast_isCongr => a.cast h
 
-theorem IsCongr.hmul_hmul {a' : Finperm n'} {b' : Finperm m'} (hab : a.IsCongr b)
+theorem IsCongr.hmul_hmul {a' : PermVector n'} {b' : PermVector m'} (hab : a.IsCongr b)
     (hab' : a'.IsCongr b') : (a.hmul a').IsCongr (b.hmul b') :=
   IsCongr.mul_mul (by simp [hab]) (by simp [hab'])
 
 grind_pattern IsCongr.hmul_hmul => a.hmul a', b.hmul b'
 
-instance : Setoid (Σ n, Finperm n) where
+def sigmaSetoid : Setoid (Σ n, PermVector n) where
   r a b := a.2.IsCongr b.2
   iseqv := by grind [Equivalence]
 
 section MinPerm
 
-variable {n m : Nat} (a : Finperm n) (b : Finperm m)
+variable {n m : Nat} (a : PermVector n) (b : PermVector m)
 
 @[grind →] theorem IsCongr.minLen_eq (hab : a.IsCongr b) :
     a.minLen = b.minLen := by rcases hab <;> grind
@@ -162,4 +162,6 @@ end MinPerm
 
 end IsCongr
 
-end Finperm
+end PermVector
+
+def FinitePerm := Quotient PermVector.sigmaSetoid
