FinitePerm/HMul.lean
@@ -4,18 +4,18 @@ Released under Apache 2.0 license as described in the file LICENSE.
 Authors: Wrenna Robson
 -/
 module
-public import Finperm.Cast
+public import FinitePerm.Cast
 
 @[expose] public section
 
-namespace Finperm
+namespace PermVector
 
-def hmul {m n : Nat} (a : Finperm m) (b : Finperm n) : Finperm (max m n) :=
+def hmul {m n : Nat} (a : PermVector m) (b : PermVector n) : PermVector (max m n) :=
   a.castGE (Nat.le_max_left m n) * b.castGE (Nat.le_max_right m n)
 
 section HMul
 
-variable {m n : Nat} (a : Finperm m) (b : Finperm n)
+variable {m n : Nat} (a : PermVector m) (b : PermVector n)
 
 @[simp, grind =] theorem getElem_hmul {i : Nat} (hi : i < max m n) :
     (a.hmul b)[i] = if hn : i < n then if hm : b[i] < m then a[b[i]] else b[i]
@@ -33,7 +33,7 @@ theorem getElem_inv_hmul {i : Nat} (hi : i < max m n) :
   grind [getElem_inv_hmul]
 
 @[simp, grind =]
-theorem hmul_eq_mul {a b : Finperm n} : a.hmul b = (a * b).cast (Nat.max_self n).symm := by
+theorem hmul_eq_mul {a b : PermVector n} : a.hmul b = (a * b).cast (Nat.max_self n).symm := by
   ext
   simp only [getElem_hmul, getElem_lt, getElem_cast]
   grind
@@ -54,4 +54,4 @@ theorem hmul_castGE_right {k : Nat} (h : n ≤ k) :
 
 end HMul
 
-end Finperm
+end PermVector
