FinitePerm.lean
@@ -1,0 +1,7 @@
+-- This module serves as the root of the `FinitePerm` library.
+-- Import modules here that should be built as part of the library.
+import FinitePerm.Basic
+import FinitePerm.Cast
+import FinitePerm.MinPerm
+import FinitePerm.Congr
+import FinitePerm.HMul
