Finperm.lean
@@ -1,7 +1,0 @@
--- This module serves as the root of the `Finperm` library.
--- Import modules here that should be built as part of the library.
-import Finperm.Basic
-import Finperm.Cast
-import Finperm.MinPerm
-import Finperm.Congr
-import Finperm.HMul
